Clean up of translations

coq/NNRC/Optim/NNRCOptimizer.v
@@ -18,20 +18,29 @@
 
 Section NNRCOptimizer.
   Require Import String.
-  Require Import List.
+  Require Import List ListSet.
   Require Import Arith.
-  
-  Require Import Utils BasicRuntime.
-  Require Import NNRCSystem.
-  Require Import NNRCRewriteUtil NNRCRewrite.
-
+  Require Import Equivalence.
+  Require Import Morphisms.
+  Require Import Setoid.
+  Require Import EquivDec.
   Require Import Program.
 
-  Context {fruntime:foreign_runtime}.
+  Require Import Utils BasicSystem.
+  Require Import NNRCSystem.
+  Require Import NNRCRewriteUtil NNRCRewrite TNNRCRewrite.
+  Require Import OptimizerLogger.
+  Require Import OptimizerStep.
 
-  (** Apply the function f to the direct child of p *)
-  Definition nnrc_map (f: nnrc -> nnrc) (e:nnrc) :=
-    match e with
+  Local Open Scope nnrc_scope.
+  Local Open Scope string.
+
+  Section engine.
+    (** Apply the function f to the direct child of p *)
+    Context {fruntime:foreign_runtime}.
+
+    Definition nnrc_map (f: nnrc -> nnrc) (e:nnrc) :=
+      match e with
       | NNRCVar v => NNRCVar v
       | NNRCConst d => NNRCConst d
       | NNRCBinop bop e1 e2 => NNRCBinop bop (f e1) (f e2)
@@ -41,21 +50,21 @@ Section NNRCOptimizer.
       | NNRCIf e1 e2 e3 => NNRCIf (f e1) (f e2) (f e3)
       | NNRCEither ed xl el xr er => NNRCEither (f ed) xl (f el) xr (f er)
       | NNRCGroupBy g sl e1 => NNRCGroupBy g sl (f e1)
-    end.
+      end.
 
-  Lemma nnrc_map_correctness:
-    forall f: nnrc -> nnrc,
-    forall e: nnrc,
-      (forall e', nnrc_ext_eq (f e') e') -> nnrc_ext_eq (nnrc_map f e) e.
-  Proof.
-    intros f e Hf.
-    nnrc_cases (induction e) Case;
-      try solve [simpl; repeat rewrite Hf; reflexivity].
-  Qed.
+    Lemma nnrc_map_correctness:
+      forall f: nnrc -> nnrc,
+      forall e: nnrc,
+        (forall e', nnrc_ext_eq (f e') e') -> nnrc_ext_eq (nnrc_map f e) e.
+    Proof.
+      intros f e Hf.
+      nnrc_cases (induction e) Case;
+        try solve [simpl; repeat rewrite Hf; reflexivity].
+    Qed.
 
-  (** Apply the function f to all subexpression of e. *)
-  Fixpoint nnrc_map_deep (f: nnrc -> nnrc) (e: nnrc) :=
-    match e with
+    (** Apply the function f to all subexpression of e. *)
+    Fixpoint nnrc_map_deep (f: nnrc -> nnrc) (e: nnrc) :=
+      match e with
       | NNRCVar v => f (NNRCVar v)
       | NNRCConst d => f (NNRCConst d)
       | NNRCBinop bop e1 e2 => f (NNRCBinop bop (nnrc_map_deep f e1) (nnrc_map_deep f e2))
@@ -65,53 +74,1009 @@ Section NNRCOptimizer.
       | NNRCIf e1 e2 e3 => f (NNRCIf (nnrc_map_deep f e1) (nnrc_map_deep f e2) (nnrc_map_deep f e3))
       | NNRCEither ed xl el xr er => f (NNRCEither (nnrc_map_deep f ed) xl (nnrc_map_deep f  el) xr (nnrc_map_deep f er))
       | NNRCGroupBy g sl e1 => f (NNRCGroupBy g sl (nnrc_map_deep f e1))
-    end.
+      end.
 
-  Lemma nnrc_map_deep_corretness:
-    forall f: nnrc -> nnrc,
-    forall e: nnrc,
-      (forall e', nnrc_ext_eq (f e') e') -> nnrc_ext_eq (nnrc_map_deep f e) e.
-  Proof.
-    intros f e Hf.
-    nnrc_cases (induction e) Case; simpl;
-      try solve [repeat rewrite Hf; reflexivity];
-      try solve [repeat rewrite Hf; rewrite IHe; reflexivity ];
-      try solve [repeat rewrite Hf; rewrite IHe1; rewrite IHe2; reflexivity ];
-      try solve [repeat rewrite Hf; rewrite IHe1; rewrite IHe2; rewrite IHe3; reflexivity ].
-  Qed.
+    Lemma nnrc_map_deep_corretness:
+      forall f: nnrc -> nnrc,
+      forall e: nnrc,
+        (forall e', nnrc_ext_eq (f e') e') -> nnrc_ext_eq (nnrc_map_deep f e) e.
+    Proof.
+      intros f e Hf.
+      nnrc_cases (induction e) Case; simpl;
+        try solve [repeat rewrite Hf; reflexivity];
+        try solve [repeat rewrite Hf; rewrite IHe; reflexivity ];
+        try solve [repeat rewrite Hf; rewrite IHe1; rewrite IHe2; reflexivity ];
+        try solve [repeat rewrite Hf; rewrite IHe1; rewrite IHe2; rewrite IHe3; reflexivity ].
+    Qed.
 
-  (* Java equivalent: NnrcOptimizer.rew_iter *)
-(*  Definition rew_iter (rew: nnrc -> nnrc) (fuel: nat) (p: nnrc)
+    (* Java equivalent: NnrcOptimizer.rew_iter *)
+    (*  Definition rew_iter (rew: nnrc -> nnrc) (fuel: nat) (p: nnrc)
     := iter rew fuel p.
-*)
-  (* Java equivalent: NnrcOptimizer.rew_size *)
-  (* Definition rew_size (rew: nnrc -> nnrc) (p: nnrc) :=
+     *)
+    (* Java equivalent: NnrcOptimizer.rew_size *)
+    (* Definition rew_size (rew: nnrc -> nnrc) (p: nnrc) :=
     iter_cost rew NNRCSize.nnrc_size p.
-   *)
-  (* *************************** *)
+     *)
+    (* *************************** *)
 
-  (* unshadowing *)
+    (* unshadowing *)
 
-  Definition nunshadow := unshadow_simpl nil.
+    Definition nunshadow := unshadow_simpl nil.
   
-  (* *************************** *)
-  Definition head_rew (e: nnrc) :=
-    (nunshadow e).
-
-  Lemma head_rew_correctness e:
-    nnrc_ext_eq (head_rew e) e.
-  Proof.
-    unfold head_rew.
+    (* *************************** *)
+    Definition head_rew (e: nnrc) :=
+      (nunshadow e).
+    
+    Lemma head_rew_correctness e:
+      nnrc_ext_eq (head_rew e) e.
+    Proof.
+      unfold head_rew.
     apply unshadow_ext_preserves.
+    Qed.
+
+    Lemma rewriter_simpl_rew_no_free_var :
+      forall (op : nnrc) (x : var),
+        In x (nnrc_free_vars (head_rew op)) -> In x (nnrc_free_vars op).
+    Proof.
+      intros.
+      unfold head_rew in H.
+      eapply unshadow_free_vars; eapply H.
+    Qed.
+    (* *************************** *)
+
+  End engine.
+
+  Ltac tcorrectness_prover :=
+    simpl; repeat progress
+                  (try match goal with
+                       | [|- context [match ?p with | _ => _ end] ] => destruct p
+                       end; try reflexivity; try unfold Equivalence.equiv in *; try subst).
+  
+  Ltac tprove_correctness p :=
+    destruct p;
+    tcorrectness_prover.
+
+  Lemma tnnrc_ext_rewrites_to_trans {model:basic_model} e1 e2 e3:
+    tnnrc_ext_rewrites_to e1 e2 -> tnnrc_ext_rewrites_to e2 e3 -> tnnrc_ext_rewrites_to e1 e3.
+  Proof.
+    apply transitivity.
   Qed.
 
-  Lemma rewriter_simpl_rew_no_free_var :
-    forall (op : nnrc) (x : var),
-      In x (nnrc_free_vars (head_rew op)) -> In x (nnrc_free_vars op).
+  Lemma AUX {model:basic_model} f e e' :
+    (forall e, tnnrc_ext_rewrites_to e (f e)) -> tnnrc_ext_rewrites_to e e' -> tnnrc_ext_rewrites_to e (f e').
   Proof.
     intros.
-    unfold head_rew in H.
-    eapply unshadow_free_vars; eapply H.
+    rewrite H0 at 1.
+    rewrite (H e') at 1.
+    reflexivity.
+  Qed.
+
+  Definition tnnrc_map {fruntime:foreign_runtime} := nnrc_map.
+
+  Lemma tnnrc_map_correctness {model:basic_model}:
+    forall f: nnrc -> nnrc,
+    forall p: nnrc,
+      (forall p', tnnrc_ext_rewrites_to p' (f p')) -> tnnrc_ext_rewrites_to p (tnnrc_map f p).
+  Proof.
+    intros.
+    nnrc_cases (induction p) Case; try solve [simpl; apply Hf]; simpl;
+    try reflexivity;
+    try (rewrite (H p1) at 1; rewrite (H p2) at 1; reflexivity).
+    rewrite (H p) at 1; reflexivity.
+    simpl.
+    rewrite (H p1) at 1; rewrite (H p2) at 1; rewrite (H p3) at 1.
+    reflexivity.
+    rewrite (H p1) at 1; rewrite (H p2) at 1; rewrite (H p3) at 1.
+    reflexivity.
+    rewrite (H p) at 1; reflexivity.
+  Qed.
+
+  Definition tnnrc_map_deep {fruntime:foreign_runtime} := nnrc_map_deep.
+  Lemma tnnrc_map_deep_correctness {model:basic_model}:
+    forall f: nnrc -> nnrc,
+    forall p: nnrc,
+      (forall p', tnnrc_ext_rewrites_to p' (f p')) -> tnnrc_ext_rewrites_to p (tnnrc_map_deep f p).
+  Proof.
+    intros f p Hf.
+    nnrc_cases (induction p) Case; try solve [simpl; apply Hf];
+    try reflexivity; simpl;
+    try (rewrite IHp1 at 1; rewrite IHp2 at 1; rewrite Hf at 1; reflexivity);
+    try (rewrite IHp at 1; rewrite Hf at 1; reflexivity).
+    rewrite IHp1 at 1; rewrite IHp2 at 1; rewrite IHp3 at 1; rewrite Hf at 1; reflexivity.
+    rewrite IHp1 at 1; rewrite IHp2 at 1; rewrite IHp3 at 1; rewrite Hf at 1; reflexivity.
+  Qed.
+
+  (****************)
+      
+  (* Java equivalent: NnrcOptimizer.tunshadow_preserves_fun *)
+  Definition tunshadow_preserves_fun {fruntime:foreign_runtime} (e:nnrc) :=
+    unshadow_simpl nil e.
+
+  Lemma tunshadow_preserves_fun_correctness {model:basic_model} (e:nnrc):
+    tnnrc_ext_rewrites_to e (tunshadow_preserves_fun e).
+  Proof.
+    unfold tunshadow_preserves_fun, unshadow_simpl.
+    apply tunshadow_preserves_arrow.
+  Qed.
+
+  Definition tunshadow_preserves_step {fruntime:foreign_runtime}
+    := mkOptimizerStep
+         "unshadow" (* name *)
+         "Renames variables to avoid shadowing" (* description *)
+         "tunshadow_preserves_fun" (* lemma name *)
+         tunshadow_preserves_fun (* lemma *).
+
+  Definition tunshadow_preserves_step_correct {model:basic_model}
+    := mkOptimizerStepModel tunshadow_preserves_step tunshadow_preserves_fun_correctness.
+
+
+  (* Java equivalent: NnrcOptimizer.[same] *)
+  Definition tfor_nil_fun  {fruntime:foreign_runtime}(e:nnrc) :=
+    match e with
+    | NNRCFor x ‵{||} e2 => ‵{||}
+    | _ => e
+    end.
+  
+  Lemma tfor_nil_fun_correctness {model:basic_model} (e:nnrc) :
+    tnnrc_ext_rewrites_to e (tfor_nil_fun e).
+  Proof.
+    tprove_correctness e.
+    apply tfor_nil_arrow.
+  Qed.
+
+  Definition tfor_nil_step {fruntime:foreign_runtime}
+    := mkOptimizerStep
+         "for/nil" (* name *)
+         "Remove loop comprehensions over empty bags" (* description *)
+         "tfor_nil_fun" (* lemma name *)
+         tfor_nil_fun (* lemma *).
+
+  Definition tfor_nil_step_correct {model:basic_model}
+    := mkOptimizerStepModel tfor_nil_step tfor_nil_fun_correctness.
+
+  (* Java equivalent: NnrcOptimizer.[same] *)
+  Definition tfor_singleton_to_let_fun  {fruntime:foreign_runtime} (e:nnrc) :=
+    match e with
+    | NNRCFor x (NNRCUnop AColl e1) e2
+      => NNRCUnop AColl (NNRCLet x e1 e2)
+    | _ => e
+    end.
+
+  Lemma tfor_singleton_to_let_fun_correctness {model:basic_model} (e:nnrc) :
+    tnnrc_ext_rewrites_to e (tfor_singleton_to_let_fun e).
+  Proof.
+    tprove_correctness e.
+    apply tfor_singleton_to_let_arrow.
+  Qed.
+
+  Definition tfor_singleton_to_let_step {fruntime:foreign_runtime}
+    := mkOptimizerStep
+         "for/singleton" (* name *)
+         "Lower a loop comprehension over a singleton into a singleton of a let" (* description *)
+         "tfor_singleton_to_let_step" (* lemma name *)
+         tfor_singleton_to_let_fun (* lemma *).
+  
+  Definition tfor_singleton_to_let_step_correct {model:basic_model}
+    := mkOptimizerStepModel tfor_singleton_to_let_step tfor_singleton_to_let_fun_correctness.
+
+  (* Java equivalent: NnrcOptimizer.[same] *)
+  Definition tflatten_singleton_fun  {fruntime:foreign_runtime} (e:nnrc)
+    := match e with
+       | ♯flatten(‵{| e1 |}) => e1
+       | _ => e
+       end.
+
+  Lemma tflatten_singleton_fun_correctness {model:basic_model} (e:nnrc) :
+    tnnrc_ext_rewrites_to e (tflatten_singleton_fun e).
+  Proof.
+    tprove_correctness e.
+    apply tflatten_singleton_nnrc_arrow.
+  Qed.
+
+  Definition tflatten_singleton_step {fruntime:foreign_runtime}
+    := mkOptimizerStep
+         "flatten/singleton" (* name *)
+         "Simplify a flatten of a singleton bag" (* description *)
+         "tflatten_singleton_fun" (* lemma name *)
+         tflatten_singleton_fun (* lemma *).
+  
+  Definition tflatten_singleton_step_correct {model:basic_model}
+    := mkOptimizerStepModel tflatten_singleton_step tflatten_singleton_fun_correctness.
+
+  (* Java equivalent: NnrcOptimizer.[same] *)
+  Definition tflatten_nil_fun  {fruntime:foreign_runtime} (e:nnrc)
+    := match e with
+       | ♯flatten(‵{||}) => ‵{||}
+       | _ => e
+       end.
+
+  Lemma tflatten_nil_fun_correctness {model:basic_model} (e:nnrc) :
+    tnnrc_ext_rewrites_to e (tflatten_nil_fun e).
+  Proof.
+    tprove_correctness e.
+    apply tflatten_nil_nnrc_arrow.
+  Qed.
+
+  Definition tflatten_nil_step {fruntime:foreign_runtime}
+    := mkOptimizerStep
+         "flatten/nil" (* name *)
+         "Simplify flatten of an empty bag" (* description *)
+         "tflatten_nil_fun" (* lemma name *)
+         tflatten_nil_fun (* lemma *).
+  
+  Definition tflatten_nil_step_correct {model:basic_model}
+    := mkOptimizerStepModel tflatten_nil_step tflatten_nil_fun_correctness.
+
+  Definition tsigma_to_if_fun  {fruntime:foreign_runtime}(e:nnrc) :=
+    match e with
+      | (NNRCUnop AFlatten
+                 (NNRCFor v1 (NNRCUnop AColl e2)
+                         (NNRCIf e1
+                                (NNRCUnop AColl (NNRCVar v2))
+                                (NNRCConst (dcoll nil))))) =>
+        if (v1 == v2)
+        then (NNRCLet v1 e2 (NNRCIf e1 (NNRCUnop AColl (NNRCVar v1)) (NNRCConst (dcoll nil))))
+        else e
+      | _ => e
+    end.
+
+  (* ♯flatten({ e1 ? { $t1 } : {} | $t1 ∈ { e2 } }) ≡ LET $t1 := e2 IN e1 ? { $t1 } : {} *)
+
+  Lemma tsigma_to_if_fun_correctness {model:basic_model} (e:nnrc) :
+    tnnrc_ext_rewrites_to e (tsigma_to_if_fun e).
+  Proof.
+    tprove_correctness e.
+    apply tsigma_to_if_arrow.
+  Qed.
+
+  Definition tsigma_to_if_step {fruntime:foreign_runtime}
+    := mkOptimizerStep
+         "sigma/if" (* name *)
+         "???" (* description *)
+         "tsigma_to_if_fun" (* lemma name *)
+         tsigma_to_if_fun (* lemma *).
+
+  Definition tsigma_to_if_step_correct {model:basic_model}
+    := mkOptimizerStepModel tsigma_to_if_step tsigma_to_if_fun_correctness.
+  
+  (* {| e3 | $t2 ∈ ♯flatten({| e2 ? ‵{|$t1|} : ‵{||} | $t1 ∈ e1 |}) |}
+       ⇒ ♯flatten({| e2 ? ‵{| LET $t2 := $t1 IN e3 ]|} : ‵{||} | $t1 ∈ e1 |}) *)
+
+  (* Java equivalent: NnrcOptimizer.[same] *)
+  Definition tmap_sigma_fusion_samevar_fun  {fruntime:foreign_runtime}(e:nnrc) :=
+    match e with
+      | (NNRCFor v2 
+                (NNRCUnop AFlatten
+                         (NNRCFor v1 e1
+                                 (NNRCIf e2 (NNRCUnop AColl (NNRCVar v1')) (NNRCConst (dcoll nil)))))
+                e3) =>
+        if (v1 == v1')
+        then
+          if (v1 == v2)
+          then
+            (NNRCUnop AFlatten
+                     (NNRCFor v1 e1
+                             (NNRCIf e2
+                                    (NNRCUnop AColl e3)
+                                    (NNRCConst (dcoll nil)))))
+          else e
+        else e
+      | _ => e
+    end.
+
+  Lemma tmap_sigma_fusion_samevar_fun_correctness {model:basic_model} (e:nnrc) :
+    tnnrc_ext_rewrites_to e (tmap_sigma_fusion_samevar_fun e).
+  Proof.
+    tprove_correctness e.
+    apply tmap_sigma_fusion_samevar_arrow.
+  Qed.
+
+    Definition tmap_sigma_fusion_samevar_step {fruntime:foreign_runtime}
+    := mkOptimizerStep
+         "sigma/same var fusion" (* name *)
+         "???" (* description *)
+         "tmap_sigma_fusion_samevar_fun" (* lemma name *)
+         tmap_sigma_fusion_samevar_fun (* lemma *).
+
+  Definition tmap_sigma_fusion_samevar_step_correct {model:basic_model}
+    := mkOptimizerStepModel tmap_sigma_fusion_samevar_step tmap_sigma_fusion_samevar_fun_correctness.
+
+  (* Java equivalent: NnrcOptimizer.[same] *)
+  Definition tdot_of_rec_fun  {fruntime:foreign_runtime}(e:nnrc) :=
+    match e with
+      | (NNRCUnop (ADot s1)
+                (NNRCUnop (ARec s2) e1)) =>
+        if (s1 == s2)
+        then e1
+        else e
+      | _ => e
+    end.
+
+  Lemma tdot_of_rec_fun_correctness {model:basic_model} (e:nnrc) :
+    tnnrc_ext_rewrites_to e (tdot_of_rec_fun e).
+  Proof.
+    tprove_correctness e.
+    apply tdot_of_rec.
+  Qed.
+
+    Definition tdot_of_rec_step {fruntime:foreign_runtime}
+    := mkOptimizerStep
+         "dot/rec" (* name *)
+         "Simplify lookup of a new record constructor" (* description *)
+         "tdot_of_rec_fun" (* lemma name *)
+         tdot_of_rec_fun (* lemma *).
+
+  Definition tdot_of_rec_step_correct {model:basic_model}
+    := mkOptimizerStepModel tdot_of_rec_step tdot_of_rec_fun_correctness.
+
+  (* Java equivalent: NnrcOptimizer.[same] *)
+  Definition tmerge_concat_to_concat_fun  {fruntime:foreign_runtime}(e:nnrc)
+    := match e with
+       | (‵[| (s1, p1)|] ⊗ ‵[| (s2, p2)|])
+         => if (equiv_decb s1 s2)
+            then e
+            else (‵{|‵[| (s1, p1)|] ⊕ ‵[| (s2, p2)|]|})
+       | _ => e
+       end.
+
+  Lemma tmerge_concat_to_concat_fun_correctness {model:basic_model} (e:nnrc) :
+    tnnrc_ext_rewrites_to e (tmerge_concat_to_concat_fun e).
+  Proof.
+    destruct e; simpl; try reflexivity.
+    destruct b; simpl; try reflexivity.
+    destruct e1; simpl; try reflexivity.
+    destruct u; simpl; try reflexivity.
+    destruct e2; simpl; try reflexivity.
+    destruct u; simpl; try reflexivity.
+    unfold equiv_decb.
+    destruct (equiv_dec s s0); try reflexivity.
+    apply tnnrc_merge_concat_to_concat_arrow; trivial.
+  Qed.
+
+    Definition tmerge_concat_to_concat_step {fruntime:foreign_runtime}
+    := mkOptimizerStep
+         "merge-concat->merge" (* name *)
+         "Simplify a merge-concat of two singleton records with different fields using concat" (* description *)
+         "tmerge_concat_to_concat_fun" (* lemma name *)
+         tmerge_concat_to_concat_fun (* lemma *).
+
+  Definition tmerge_concat_to_concat_step_correct {model:basic_model}
+    := mkOptimizerStepModel tmerge_concat_to_concat_step tmerge_concat_to_concat_fun_correctness.
+
+  (* Java equivalent: NnrcOptimizer.[same] *)
+  Definition tdot_of_concat_rec_fun  {fruntime:foreign_runtime}(e:nnrc)
+    := match e with
+       | (NNRCUnop (ADot s) (NNRCBinop AConcat e1 (NNRCUnop (ARec s2) e2)))
+         => if equiv_decb s s2
+            then e2
+            else (NNRCUnop (ADot s) e1)
+       | _ => e
+       end.
+
+  Lemma tdot_of_concat_rec_fun_correctness {model:basic_model} (e:nnrc) :
+    tnnrc_ext_rewrites_to e (tdot_of_concat_rec_fun e).
+  Proof.
+    destruct e; simpl; try reflexivity.
+    destruct u; simpl; try reflexivity.
+    destruct e; simpl; try reflexivity.
+    destruct b; simpl; try reflexivity.
+    destruct e2; simpl; try reflexivity.
+    destruct u; simpl; try reflexivity.
+    unfold equiv_decb.
+    destruct (equiv_dec s s0); try reflexivity.
+    - red in e; subst.
+      apply tnnrc_dot_of_concat_rec_eq_arrow.
+    - apply tnnrc_dot_of_concat_rec_neq_arrow.
+      trivial.
+  Qed.
+
+    Definition tdot_of_concat_rec_step {fruntime:foreign_runtime}
+    := mkOptimizerStep
+         "dot/concat/rec 2" (* name *)
+         "Simplifies lookup of a concatenation with a record constructor" (* description *)
+         "tdot_of_concat_rec_fun" (* lemma name *)
+         tdot_of_concat_rec_fun (* lemma *).
+
+  Definition tdot_of_concat_rec_step_correct {model:basic_model}
+    := mkOptimizerStepModel tdot_of_concat_rec_step tdot_of_concat_rec_fun_correctness.
+
+  (** Inlining *)
+
+  (* TODO: A better/less hacky cost function.  This will probably need many more real
+     examples to tune with, as it will always contain some black-magic. *)
+  (* Java equivalent: NnrcOptimizer.is_small_unop *)
+  Definition is_small_unop {fruntime:foreign_runtime} (u:unaryOp) :=
+    match u with
+    | AIdOp
+    | ANeg
+    | AColl
+    | ALeft
+    | ARight
+    | ABrand _
+    | ARec _
+      => true
+    | _ => false
+    end.
+  
+  (* Java equivalent: NnrcOptimizer.should_inline_small *)
+  Fixpoint should_inline_small {fruntime:foreign_runtime} (from:nnrc)
+    := match from with
+       | NNRCVar _
+       | NNRCConst _ => true
+       | NNRCUnop u e => is_small_unop u && should_inline_small e
+       | NNRCBinop AConcat (NNRCUnop (ARec _) e1) (NNRCUnop (ARec _) e2) => true
+       | _ => false
+       end.
+
+  (* Java equivalent: NnrcOptimizer.should_inline_few_occurances *)
+  Definition should_inline_few_occurences {fruntime:foreign_runtime} (x:var) (to:nnrc)
+    := match use_count x to with
+       | NotUsed
+       | UsedOnce => true
+       | _ => false
+       end.
+  
+  (* Java equivalent: NnrcOptimizer.should_inline *)
+  Definition should_inline {fruntime:foreign_runtime} (x:var) (from to:nnrc)
+    := should_inline_small from
+       || should_inline_few_occurences x to.
+  
+  (* Java equivalent: NnrcOptimizer.[same] *)
+  Definition tinline_let_fun  {fruntime:foreign_runtime}(e:nnrc)
+    := match e with
+       | NNRCLet x e1 e2 =>
+         if should_inline x e1 e2
+         then nnrc_subst (unshadow_simpl (nnrc_free_vars e1) e2) x e1
+         else e
+       | _ => e
+       end.
+
+  Lemma tinline_let_fun_correctness {model:basic_model} (e:nnrc) :
+    tnnrc_ext_rewrites_to e (tinline_let_fun e).
+  Proof.
+    tprove_correctness e.
+    apply tlet_inline_arrow.
+  Qed.
+
+    Definition tinline_let_step {fruntime:foreign_runtime}
+    := mkOptimizerStep
+         "let inline" (* name *)
+         "Inline let statements heuristically deemed suitable for inlining" (* description *)
+         "tinline_let_fun" (* lemma name *)
+         tinline_let_fun (* lemma *).
+
+  Definition tinline_let_step_correct {model:basic_model}
+    := mkOptimizerStepModel tinline_let_step tinline_let_fun_correctness.
+
+
+  (* push map through either and if *)
+  (* Java equivalent: NnrcOptimizer.[same] *)
+    Definition tfor_over_if_nil_fun  {fruntime:foreign_runtime}(e:nnrc)
+      := match e with
+         | NNRCFor x (NNRCIf e1 e2 ‵{||}) ebody =>
+                     (NNRCIf e1 (NNRCFor x e2 ebody) ‵{||})
+       | _ => e
+       end.
+
+  Lemma tfor_over_if_nil_fun_correctness {model:basic_model} (e:nnrc) :
+    tnnrc_ext_rewrites_to e (tfor_over_if_nil_fun e).
+  Proof.
+    tprove_correctness e.
+    rewrite tfor_over_if_arrow; simpl.
+    rewrite tfor_nil_arrow.
+    reflexivity.
+  Qed.
+
+    Definition tfor_over_if_nil_step {fruntime:foreign_runtime}
+    := mkOptimizerStep
+         "for/if/else nil" (* name *)
+         "Push loop comprehension over an if statement through the if statement when the else clause just constructs an empty bag" (* description *)
+         "tfor_over_if_nil_fun" (* lemma name *)
+         tfor_over_if_nil_fun (* lemma *).
+
+  Definition tfor_over_if_nil_step_correct {model:basic_model}
+    := mkOptimizerStepModel tfor_over_if_nil_step tfor_over_if_nil_fun_correctness.
+
+  
+  (* Java equivalent: NnrcOptimizer.[same] *)
+  Definition tfor_over_either_nil_fun  {fruntime:foreign_runtime} (e:nnrc)
+    := match e with
+       |  (NNRCFor x (NNRCEither e1 xl el xr ‵{||}) ebody)
+          => 
+            (    let xl' := really_fresh_in nnrc_unshadow_sep xl (nnrc_free_vars el ++ nnrc_bound_vars el) ebody in
+              (NNRCEither e1
+                       xl' (NNRCFor x (nnrc_subst el xl (NNRCVar xl')) ebody)
+                       xr ‵{||}))
+       | _ => e
+       end.
+
+  Lemma tfor_over_either_nil_fun_correctness {model:basic_model} (e:nnrc) :
+    tnnrc_ext_rewrites_to e (tfor_over_either_nil_fun e).
+  Proof.
+    tprove_correctness e.
+    rewrite tfor_over_either_arrow; simpl.
+    rewrite tfor_nil_arrow.
+    rewrite tnnrceither_rename_r_arrow by intuition; simpl.
+    reflexivity.
+  Qed.
+
+    Definition tfor_over_either_nil_step {fruntime:foreign_runtime}
+    := mkOptimizerStep
+         "for/either/right nil" (* name *)
+         "Push loop comprehension over an either statement through the either statement when the right clause just constructs an empty bag" (* description *)
+         "tfor_over_either_nil_fun" (* lemma name *)
+         tfor_over_either_nil_fun (* lemma *).
+
+  Definition tfor_over_either_nil_step_correct {model:basic_model}
+    := mkOptimizerStepModel tfor_over_either_nil_step tfor_over_either_nil_fun_correctness.
+
+  (* Java equivalent: NnrcOptimizer.[same] *)
+  Definition tunop_over_either_const_fun  {fruntime:foreign_runtime}(e:nnrc)
+    := match e with
+       | NNRCUnop op (NNRCEither e1 xl el xr (NNRCConst d)) =>
+         NNRCEither e1 xl (NNRCUnop op el) xr (NNRCUnop op (NNRCConst d))
+       | _ => e
+       end.
+
+  Lemma tunop_over_either_const_fun_correctness {model:basic_model} (e:nnrc) :
+    tnnrc_ext_rewrites_to e (tunop_over_either_const_fun e).
+  Proof.
+    tprove_correctness e.
+    apply tnnrcunop_over_either_arrow.
+  Qed.
+
+    Definition tunop_over_either_const_step {fruntime:foreign_runtime}
+    := mkOptimizerStep
+         "unary/either/right const" (* name *)
+         "Push unary operators through either when the right branch is a constant" (* description *)
+         "tunop_over_either_const_fun" (* lemma name *)
+         tunop_over_either_const_fun (* lemma *).
+
+  Definition tunop_over_either_const_step_correct {model:basic_model}
+    := mkOptimizerStepModel tunop_over_either_const_step tunop_over_either_const_fun_correctness.
+
+  (* Java equivalent: NnrcOptimizer.[same] *)
+  Definition tunop_over_if_const_fun  {fruntime:foreign_runtime}(e:nnrc)
+    := match e with
+       | NNRCUnop op (NNRCIf e1 e2 (NNRCConst d)) =>
+         NNRCIf e1 (NNRCUnop op e2) (NNRCUnop op (NNRCConst d))
+       | _ => e
+       end.
+
+  Lemma tunop_over_if_const_fun_correctness {model:basic_model} (e:nnrc) :
+    tnnrc_ext_rewrites_to e (tunop_over_if_const_fun e).
+  Proof.
+    tprove_correctness e.
+    apply tnnrcunop_over_if_arrow.
+  Qed.
+  
+  Definition tunop_over_if_const_step {fruntime:foreign_runtime}
+    := mkOptimizerStep
+         "unary/if/else const" (* name *)
+         "Push unary operators through if when the else branch is a constant" (* description *)
+         "tunop_over_if_const_fun" (* lemma name *)
+         tunop_over_if_const_fun (* lemma *).
+
+  Definition tunop_over_if_const_step_correct {model:basic_model}
+    := mkOptimizerStepModel tunop_over_if_const_step tunop_over_if_const_fun_correctness.
+
+    (* optimizations for rproject *)
+
+  (* Java equivalent: NnrcOptimizer.[same] *)
+   Definition tproject_nil_fun {fruntime:foreign_runtime} (e:nnrc) :=
+    match e with
+      | NNRCUnop (ARecProject nil) e₁
+        => NNRCConst (drec nil)
+      | _ => e
+    end.
+
+  Definition tproject_nil_fun_correctness {model:basic_model} p :
+    p ⇒ᶜ tproject_nil_fun p.
+  Proof.
+    tprove_correctness p.
+    apply tnnrcproject_nil.
+  Qed.
+
+  Hint Rewrite @tproject_nil_fun_correctness : toptim_correct.
+
+    Definition tproject_nil_step {fruntime:foreign_runtime}
+    := mkOptimizerStep
+         "project/nil" (* name *)
+         "Simplify record projection over empty bags" (* description *)
+         "tproject_nil_fun" (* lemma name *)
+         tproject_nil_fun (* lemma *).
+
+  Definition tproject_nil_step_correct {model:basic_model}
+    := mkOptimizerStepModel tproject_nil_step tproject_nil_fun_correctness.
+
+  (* Java equivalent: NnrcOptimizer.[same] *)
+  Definition tproject_over_const_fun {fruntime:foreign_runtime} (e:nnrc) :=
+    match e with
+      | NNRCUnop (ARecProject sl)
+          (NNRCConst (drec l))
+        => NNRCConst (drec (rproject l sl))
+      | _ => e
+    end.
+
+  Definition tproject_over_const_fun_correctness {model:basic_model} p :
+    p ⇒ᶜ tproject_over_const_fun p.
+  Proof.
+    tprove_correctness p.
+    apply tnnrcproject_over_const.
+  Qed.
+
+  Hint Rewrite @tproject_over_const_fun_correctness : toptim_correct.
+  
+  Definition tproject_over_const_step {fruntime:foreign_runtime}
+    := mkOptimizerStep
+         "project/const rec" (* name *)
+         "Simplify record projection over constant records" (* description *)
+         "tproject_over_const_fun" (* lemma name *)
+         tproject_over_const_fun (* lemma *).
+
+  Definition tproject_over_const_step_correct {model:basic_model}
+    := mkOptimizerStepModel tproject_over_const_step tproject_over_const_fun_correctness.
+  
+  (* Java equivalent: NnrcOptimizer.[same] *)
+  Definition tproject_over_rec_fun {fruntime:foreign_runtime} (e:nnrc) :=
+    match e with
+      | NNRCUnop (ARecProject sl)
+          (NNRCUnop (ARec s) p₁)
+        => if in_dec string_dec s sl
+           then NNRCUnop (ARec s) p₁
+           else ‵[||]
+      | _ => e
+    end.
+
+  Definition tproject_over_rec_fun_correctness {model:basic_model} p :
+    p ⇒ᶜ tproject_over_rec_fun p.
+  Proof.
+    tprove_correctness p.
+    - apply tnnrcproject_over_rec_in; trivial.
+    - apply tnnrcproject_over_rec_nin; trivial. 
+  Qed.
+
+  Hint Rewrite @tproject_over_rec_fun_correctness : toptim_correct.
+
+  Definition tproject_over_rec_step {fruntime:foreign_runtime}
+    := mkOptimizerStep
+         "project/rec" (* name *)
+         "Simplify record projection over a record constructor" (* description *)
+         "tproject_over_rec_fun" (* lemma name *)
+         tproject_over_rec_fun (* lemma *).
+
+  Definition tproject_over_rec_step_correct {model:basic_model}
+    := mkOptimizerStepModel tproject_over_rec_step tproject_over_rec_fun_correctness.
+
+  (* Java equivalent: NnrcOptimizer.[same] *)
+   Definition tproject_over_concat_r_fun {fruntime:foreign_runtime} (e:nnrc) :=
+    match e with
+      | NNRCUnop (ARecProject sl)
+               (NNRCBinop AConcat
+                        p₁ (NNRCUnop (ARec s) p₂))
+        => if in_dec string_dec s sl
+           then NNRCBinop AConcat
+                         (NNRCUnop (ARecProject (remove string_dec s sl)) p₁)
+                        (NNRCUnop (ARec s) p₂)
+           else (NNRCUnop (ARecProject sl) p₁)
+      | _ => e
+    end.
+
+  Definition tproject_over_concat_r_fun_correctness {model:basic_model} p :
+    p ⇒ᶜ tproject_over_concat_r_fun p.
+  Proof.
+    tprove_correctness p.
+    - apply tnnrcproject_over_concat_rec_r_in; trivial.
+    - apply tnnrcproject_over_concat_rec_r_nin; trivial.
+  Qed.
+                  
+  Hint Rewrite @tproject_over_concat_r_fun_correctness : toptim_correct.
+
+  Definition tproject_over_concat_r_step {fruntime:foreign_runtime}
+    := mkOptimizerStep
+         "project/concat/right rec" (* name *)
+         "Simplify record projection over concatenation with a record constructor" (* description *)
+         "tproject_over_concat_r_fun" (* lemma name *)
+         tproject_over_concat_r_fun (* lemma *).
+
+  Definition tproject_over_concat_r_step_correct {model:basic_model}
+    := mkOptimizerStepModel tproject_over_concat_r_step tproject_over_concat_r_fun_correctness.
+  
+  (* Java equivalent: NnrcOptimizer.[same] *)
+     Definition tproject_over_concat_l_fun {fruntime:foreign_runtime} (e:nnrc) :=
+    match e with
+      | NNRCUnop (ARecProject sl)
+               (NNRCBinop AConcat
+                        (NNRCUnop (ARec s) p₁) p₂)
+        => if in_dec string_dec s sl
+                     (* this case would need shape/type inference to handle, since we don't know if s is in p₂ *)
+
+           then e
+           else (NNRCUnop (ARecProject sl) p₂)
+      | _ => e
+    end.
+
+  Definition tproject_over_concat_l_fun_correctness {model:basic_model} p :
+    p ⇒ᶜ tproject_over_concat_l_fun p.
+  Proof.
+    tprove_correctness p.
+    apply tnnrcproject_over_concat_rec_l_nin; trivial.
+  Qed.
+                  
+  Hint Rewrite @tproject_over_concat_l_fun_correctness : toptim_correct.
+
+  Definition tproject_over_concat_l_step {fruntime:foreign_runtime}
+    := mkOptimizerStep
+         "project/concat/left rec" (* name *)
+         "Simplify record projection over concatenation with a record constructor" (* description *)
+         "tproject_over_concat_l_fun" (* lemma name *)
+         tproject_over_concat_l_fun (* lemma *).
+
+  Definition tproject_over_concat_l_step_correct {model:basic_model}
+    := mkOptimizerStepModel tproject_over_concat_l_step tproject_over_concat_l_fun_correctness.
+
+  (* Java equivalent: NnrcOptimizer.[same] *)
+  Definition tproject_over_project_fun {fruntime:foreign_runtime} (e:nnrc) :=
+    match e with
+      | NNRCUnop (ARecProject sl1)
+          (NNRCUnop (ARecProject sl2) p1)
+        => NNRCUnop (ARecProject (set_inter string_dec sl2 sl1)) p1
+      | _ => e
+    end.
+
+  Definition tproject_over_project_fun_correctness {model:basic_model} p :
+    p ⇒ᶜ tproject_over_project_fun p.
+  Proof.
+    tprove_correctness p.
+    apply tnnrcproject_over_nnrcproject.
+  Qed.
+
+  Hint Rewrite @tproject_over_project_fun_correctness : toptim_correct.
+
+  Definition tproject_over_project_step {fruntime:foreign_runtime}
+    := mkOptimizerStep
+         "project/project" (* name *)
+         "Fuse nested record projections" (* description *)
+         "tproject_over_project_fun" (* lemma name *)
+         tproject_over_project_fun (* lemma *).
+
+  Definition tproject_over_project_step_correct {model:basic_model}
+    := mkOptimizerStepModel tproject_over_project_step tproject_over_project_fun_correctness.
+
+  (* Java equivalent: NnrcOptimizer.[same] *)
+   Definition tproject_over_either_fun {fruntime:foreign_runtime} (e:nnrc) :=
+    match e with
+      | NNRCUnop (ARecProject sl)
+          (NNRCEither p xl p₁ xr p₂)
+        => NNRCEither p xl (NNRCUnop (ARecProject sl) p₁) xr (NNRCUnop (ARecProject sl) p₂)
+      | _ => e
+    end.
+
+  Definition tproject_over_either_fun_correctness {model:basic_model} p :
+    p ⇒ᶜ tproject_over_either_fun p.
+  Proof.
+    tprove_correctness p.
+    apply tnnrcproject_over_either.
+  Qed.
+
+  Hint Rewrite @tproject_over_either_fun_correctness : toptim_correct.
+
+  Definition tproject_over_either_step {fruntime:foreign_runtime}
+    := mkOptimizerStep
+         "project/either/" (* name *)
+         "Push record projection through either" (* description *)
+         "tproject_over_either_fun" (* lemma name *)
+         tproject_over_either_fun (* lemma *).
+
+  Definition tproject_over_either_step_correct {model:basic_model}
+    := mkOptimizerStepModel tproject_over_either_step tproject_over_either_fun_correctness.
+  
+  (* count optimizations *)
+  (* Java equivalent: NnrcOptimizer.[same] *)
+  Definition tcount_over_flat_for_either_if_nil_fun  {fruntime:foreign_runtime} (e:nnrc)
+    := match e with
+       | (♯count(♯flatten(NNRCFor v
+                              ehead (NNRCEither e1 xl
+                                               (NNRCIf e11(‵{| e12|}) ‵{||}) xr ‵{||}))))
+         => (♯count(♯flatten(NNRCFor v
+                              ehead (NNRCEither e1 xl
+                                               (NNRCIf e11(‵{| ‵(dunit) |}) ‵{||}) xr ‵{||}))))
+       | _ => e
+       end.
+
+  Lemma tcount_over_flat_for_either_if_nil_fun_correctness {model:basic_model} (e:nnrc) :
+    tnnrc_ext_rewrites_to e (tcount_over_flat_for_either_if_nil_fun e).
+  Proof.
+    destruct e; simpl; try reflexivity.
+    repeat (match_destr; try reflexivity).
+    apply tcount_over_flat_for_either_if_nil_arrow.
+  Qed.
+
+  Definition tcount_over_flat_for_either_if_nil_step {fruntime:foreign_runtime}
+    := mkOptimizerStep
+         "count/flatten/for/either/right if/else nil" (* name *)
+         "Remove work that is not needed when only the bag count is needed" (* description *)
+         "tcount_over_flat_for_either_if_nil_fun" (* lemma name *)
+         tcount_over_flat_for_either_if_nil_fun (* lemma *).
+
+  Definition tcount_over_flat_for_either_if_nil_step_correct {model:basic_model}
+    := mkOptimizerStepModel tcount_over_flat_for_either_if_nil_step tcount_over_flat_for_either_if_nil_fun_correctness.
+  
+  (* Java equivalent: NnrcOptimizer.[same] *)
+  Definition tcount_over_flat_for_either_either_nil_fun  {fruntime:foreign_runtime}(e:nnrc)
+    := match e with
+       | (♯count(♯flatten(NNRCFor v
+                                 ehead (NNRCEither e1 xl
+                                                  (NNRCEither e11 xll (‵{| e12|}) xrr ‵{||}) xr ‵{||}))))
+         => (♯count(♯flatten(NNRCFor v
+                                    ehead (NNRCEither e1 xl
+                                                     (NNRCEither e11 xll (‵{| ‵(dunit) |}) xrr ‵{||}) xr ‵{||}))))
+
+     | _ => e
+       end.
+
+  Lemma tcount_over_flat_for_either_either_nil_fun_correctness {model:basic_model} (e:nnrc) :
+    tnnrc_ext_rewrites_to e (tcount_over_flat_for_either_either_nil_fun e).
+  Proof.
+    destruct e; simpl; try reflexivity.
+    repeat (match_destr; try reflexivity).
+    apply tcount_over_flat_for_either_either_nil_arrow.
+  Qed.
+
+    Definition tcount_over_flat_for_either_either_nil_step {fruntime:foreign_runtime}
+    := mkOptimizerStep
+         "count/flatten/for/either/right either/right nil" (* name *)
+         "Remove work that is not needed when only the bag count is needed" (* description *)
+         "tcount_over_flat_for_either_either_nil_fun" (* lemma name *)
+         tcount_over_flat_for_either_either_nil_fun (* lemma *).
+
+  Definition tcount_over_flat_for_either_either_nil_step_correct {model:basic_model}
+    := mkOptimizerStepModel tcount_over_flat_for_either_either_nil_step tcount_over_flat_for_either_either_nil_fun_correctness.  
+                                                            
+  (* list of all optimizations *)
+    Definition tnnrc_optim_list {fruntime:foreign_runtime} : list (@OptimizerStep nnrc)
+      := [
+          tfor_nil_step
+          ; tfor_singleton_to_let_step
+          ; tflatten_singleton_step
+          ; tflatten_nil_step
+          ; tsigma_to_if_step
+          ; tmap_sigma_fusion_samevar_step
+          ; tdot_of_rec_step
+          ; tmerge_concat_to_concat_step
+          ; tdot_of_concat_rec_step
+          ; tinline_let_step
+          ; tfor_over_if_nil_step
+          ; tfor_over_either_nil_step
+          ; tunop_over_either_const_step
+          ; tunop_over_if_const_step
+          ; tproject_nil_step
+          ; tproject_over_const_step
+          ; tproject_over_rec_step
+          ; tproject_over_concat_r_step
+          ; tproject_over_concat_l_step
+          ; tproject_over_project_step
+          ; tproject_over_either_step
+          ; tcount_over_flat_for_either_if_nil_step
+          ; tcount_over_flat_for_either_either_nil_step
+        ].
+
+    Definition tnnrc_optim_model_list {model:basic_model} : list (OptimizerStepModel tnnrc_ext_rewrites_to)
+      := [
+          tfor_nil_step_correct
+          ; tfor_singleton_to_let_step_correct
+          ; tflatten_singleton_step_correct
+          ; tflatten_nil_step_correct
+          ; tsigma_to_if_step_correct
+          ; tmap_sigma_fusion_samevar_step_correct
+          ; tdot_of_rec_step_correct
+          ; tmerge_concat_to_concat_step_correct
+          ; tdot_of_concat_rec_step_correct
+          ; tinline_let_step_correct
+          ; tfor_over_if_nil_step_correct
+          ; tfor_over_either_nil_step_correct
+          ; tunop_over_either_const_step_correct
+          ; tunop_over_if_const_step_correct
+          ; tproject_nil_step_correct
+          ; tproject_over_const_step_correct
+          ; tproject_over_rec_step_correct
+          ; tproject_over_concat_r_step_correct
+          ; tproject_over_concat_l_step_correct
+          ; tproject_over_project_step_correct
+          ; tproject_over_either_step_correct
+          ; tcount_over_flat_for_either_if_nil_step_correct
+          ; tcount_over_flat_for_either_either_nil_step_correct
+        ].
+
+  Lemma tnnrc_optim_model_list_complete {model:basic_model}
+    : optim_model_list_complete tnnrc_optim_list tnnrc_optim_model_list.
+  Proof.
+    optim_correct_list_complete_prover.
+  Qed.
+
+  Definition tnnrc_optim_list_correct {model:basic_model}
+    : optim_list_correct tnnrc_ext_rewrites_to tnnrc_optim_list
+    := optim_list_correct_from_model tnnrc_optim_model_list_complete.
+
+  Lemma tnnrc_optim_list_distinct {fruntime:foreign_runtime}:
+    optim_list_distinct tnnrc_optim_list.
+  Proof.
+    apply optim_list_distinct_prover.
+    vm_compute.
+    apply eq_refl.
+  Qed.
+
+  (* *************************** *)
+  Definition run_nnrc_optims 
+             {fruntime:foreign_runtime}
+             {logger:optimizer_logger string nnrc}
+             (opc:optim_phases_config)
+    : nnrc -> nnrc :=
+    run_phases tnnrc_map_deep NNRCSize.nnrc_size tnnrc_optim_list opc.
+
+  Lemma run_nnrc_optims_correctness
+        {model:basic_model} {logger:optimizer_logger string nnrc}
+        (opc:optim_phases_config)
+        (p:nnrc) :
+    tnnrc_ext_rewrites_to p (run_nnrc_optims opc p).
+  Proof.
+    unfold run_nnrc_optims.
+    apply run_phases_correctness.
+    - intros. apply tnnrc_map_deep_correctness; auto.
+    - apply tnnrc_optim_list_correct.
+  Qed.
+
+  Section default.
+  
+    (* Java equivalent: NnrcOptimizer.head_rew_list *)
+    Definition nnrc_default_optim_list {fruntime:foreign_runtime} : list string
+    := [
+        optim_step_name tinline_let_step
+        ; optim_step_name tcount_over_flat_for_either_either_nil_step
+        ; optim_step_name tcount_over_flat_for_either_if_nil_step
+        ; optim_step_name tmerge_concat_to_concat_step
+        ; optim_step_name tdot_of_concat_rec_step
+        ; optim_step_name tdot_of_rec_step
+        ; optim_step_name tflatten_singleton_step
+        ; optim_step_name tflatten_nil_step
+        ; optim_step_name tfor_singleton_to_let_step
+        ; optim_step_name tunop_over_either_const_step
+        ; optim_step_name tunop_over_if_const_step
+        ; optim_step_name tfor_over_either_nil_step
+        ; optim_step_name tfor_over_if_nil_step
+        ; optim_step_name tfor_nil_step
+        ; optim_step_name tmap_sigma_fusion_samevar_step
+        ; optim_step_name tproject_nil_step
+        ; optim_step_name tproject_over_const_step
+        ; optim_step_name tproject_over_rec_step
+        ; optim_step_name tproject_over_concat_r_step
+        ; optim_step_name tproject_over_concat_l_step
+        ; optim_step_name tproject_over_project_step
+        ; optim_step_name tproject_over_either_step
+      ].
+    
+    Remark nnrc_default_optim_list_all_valid {fruntime:foreign_runtime}
+      : valid_optims tnnrc_optim_list nnrc_default_optim_list = (nnrc_default_optim_list,nil).
+    Proof.
+      vm_compute; trivial.
+    Qed.
+  
+    Definition default_nnrc_optim_phases {fruntime:foreign_runtime} :=
+      ("[nnrc] default"%string,nnrc_default_optim_list,10)::nil.
+
+  End default.
+  
+  (* Java equivalent: NnrcOptimizer.trew *)
+  Definition run_nnrc_optims_default
+             {fruntime:foreign_runtime} {logger:optimizer_logger string nnrc}
+    := run_nnrc_optims default_nnrc_optim_phases.
+
+  Lemma run_nnrc_optims_default_correct
+        {model:basic_model} {logger:optimizer_logger string nnrc} p:
+    tnnrc_ext_rewrites_to p (run_nnrc_optims_default p).
+  Proof.
+    unfold run_nnrc_optims_default.
+    apply run_nnrc_optims_correctness.
   Qed.
 
 End NNRCOptimizer.
